src/riot/asn1/ASN1.Low.Value.PRINTABLE_STRING.fst
@@ -4,26 +4,15 @@ open ASN1.Base
 open ASN1.Spec.Value.PRINTABLE_STRING
 open ASN1.Low.Value.StringCombinator
 open ASN1.Low.Base
-open LowParse.Low.Bytes
 
-open ASN1.Spec.Tag
-open ASN1.Spec.Length
 open ASN1.Low.Tag
 open ASN1.Low.Length
 
 open FStar.Integers
 
-module HS = FStar.HyperStack
-module HST = FStar.HyperStack.ST
-module MB = LowStar.Monotonic.Buffer
-module B = LowStar.Buffer
-module Cast = FStar.Int.Cast
+friend ASN1.Spec.Value.PRINTABLE_STRING
 
-module B32 = FStar.Bytes
-
-inline_for_extraction noextract
 let serialize32_asn1_printable_string_TLV_backwards
-: serializer32_backwards (serialize_asn1_printable_string_TLV)
 = serialize32_asn1_string_TLV_backwards
     (PRINTABLE_STRING)
     (dfst)
@@ -32,11 +21,7 @@ let serialize32_asn1_printable_string_TLV_backwards
     (synth_asn1_printable_string_inverse)
     ()
 
-inline_for_extraction noextract
-let serialize32_asn1_printable_string_TLV_with_character_bound_backwards
-  (lb: asn1_value_int32_of_type PRINTABLE_STRING)
-  (ub: asn1_value_int32_of_type PRINTABLE_STRING { lb <= ub })
-: serializer32_backwards (serialize_asn1_printable_string_TLV_with_character_bound lb ub)
+let serialize32_asn1_printable_string_TLV_with_character_bound_backwards lb ub
 = serialize32_asn1_string_TLV_with_character_bound_backwards
     (PRINTABLE_STRING)
     (dfst)
