src/riot/asn1/ASN1.Spec.Value.PRINTABLE_STRING.fst
@@ -12,25 +12,8 @@ open FStar.Integers
 
 module B32 = FStar.Bytes
 
-let filter_asn1_printable_string
-  (len: asn1_value_int32_of_type PRINTABLE_STRING)
-  (s32: B32.lbytes32 len)
-: GTot (bool)
-= let s = B32.reveal s32 in
-  Seq.for_all valid_PRINTABLE_byte s
 
-let synth_asn1_printable_string
-  (len: asn1_value_int32_of_type PRINTABLE_STRING)
-  (s32: parse_filter_refine (filter_asn1_printable_string len))
-: GTot (value: datatype_of_asn1_type PRINTABLE_STRING{(dfst value) == len})
-= (|len, s32|)
-
-noextract inline_for_extraction
-let synth_asn1_printable_string_inverse
-  (len: asn1_value_int32_of_type PRINTABLE_STRING)
-  (value: datatype_of_asn1_type PRINTABLE_STRING{(dfst value) == len})
-: Tot (s32: parse_filter_refine (filter_asn1_printable_string len)
-             { value == synth_asn1_printable_string len s32 })
+let synth_asn1_printable_string_inverse len value
 = dsnd value
 
 let parse_asn1_printable_string
@@ -41,36 +24,7 @@ let parse_asn1_printable_string
     (synth_asn1_printable_string)
     ()
 
-let serialize_asn1_printable_string
-= serialize_asn1_string
-    (PRINTABLE_STRING)
-    (dfst)
-    (filter_asn1_printable_string)
-    (synth_asn1_printable_string)
-    (synth_asn1_printable_string_inverse)
-    ()
-
-let lemma_serialize_asn1_printable_string_unfold
-= lemma_serialize_asn1_string_unfold
-    (PRINTABLE_STRING)
-    (dfst)
-    (filter_asn1_printable_string)
-    (synth_asn1_printable_string)
-    (synth_asn1_printable_string_inverse)
-    ()
-
-let lemma_serialize_asn1_printable_string_size
-= lemma_serialize_asn1_string_size
-    (PRINTABLE_STRING)
-    (dfst)
-    (filter_asn1_printable_string)
-    (synth_asn1_printable_string)
-    (synth_asn1_printable_string_inverse)
-    ()
-
-let parse_asn1_printable_string_TLV_kind = parse_asn1_string_TLV_kind PRINTABLE_STRING
 let parse_asn1_printable_string_TLV
-: parser parse_asn1_printable_string_TLV_kind (datatype_of_asn1_type PRINTABLE_STRING)
 = parse_asn1_string_TLV
     (PRINTABLE_STRING)
     (dfst)
@@ -79,7 +33,6 @@ let parse_asn1_printable_string_TLV
     ()
 
 let serialize_asn1_printable_string_TLV
-: serializer (parse_asn1_printable_string_TLV)
 = serialize_asn1_string_TLV
     (PRINTABLE_STRING)
     (dfst)
@@ -88,57 +41,7 @@ let serialize_asn1_printable_string_TLV
     (synth_asn1_printable_string_inverse)
     ()
 
-let lemma_serialize_asn1_printable_string_TLV_unfold
-  (x: datatype_of_asn1_type PRINTABLE_STRING)
-: Lemma (
-  predicate_serialize_asn1_string_TLV_unfold
-    (PRINTABLE_STRING)
-    (dfst)
-    (filter_asn1_printable_string)
-    (synth_asn1_printable_string)
-    (synth_asn1_printable_string_inverse)
-    ()
-    (x)
-)
-= lemma_serialize_asn1_string_TLV_unfold
-    (PRINTABLE_STRING)
-    (dfst)
-    (filter_asn1_printable_string)
-    (synth_asn1_printable_string)
-    (synth_asn1_printable_string_inverse)
-    ()
-    (x)
-
-let lemma_serialize_asn1_printable_string_TLV_size
-  (x: datatype_of_asn1_type PRINTABLE_STRING)
-: Lemma (
-  predicate_serialize_asn1_string_TLV_size
-    (PRINTABLE_STRING)
-    (dfst)
-    (filter_asn1_printable_string)
-    (synth_asn1_printable_string)
-    (synth_asn1_printable_string_inverse)
-    ()
-    (x)
-)
-= lemma_serialize_asn1_string_TLV_size
-    (PRINTABLE_STRING)
-    (dfst)
-    (filter_asn1_printable_string)
-    (synth_asn1_printable_string)
-    (synth_asn1_printable_string_inverse)
-    ()
-    (x)
-
-let count_printable_character
-  (x: datatype_of_asn1_type PRINTABLE_STRING)
-: Tot (asn1_int32)
-= dfst x
-
-let parse_asn1_printable_string_TLV_with_character_bound
-  (lb: asn1_value_int32_of_type PRINTABLE_STRING)
-  (ub: asn1_value_int32_of_type PRINTABLE_STRING { lb <= ub })
-: parser parse_asn1_printable_string_TLV_kind (asn1_string_with_character_bound_t PRINTABLE_STRING count_printable_character lb ub)
+let parse_asn1_printable_string_TLV_with_character_bound lb ub
 = parse_asn1_string_TLV_with_character_bound
     (PRINTABLE_STRING)
     (dfst)
@@ -149,10 +52,7 @@ let parse_asn1_printable_string_TLV_with_character_bound
     (lb)
     (ub)
 
-let serialize_asn1_printable_string_TLV_with_character_bound
-  (lb: asn1_value_int32_of_type PRINTABLE_STRING)
-  (ub: asn1_value_int32_of_type PRINTABLE_STRING { lb <= ub })
-: serializer (parse_asn1_printable_string_TLV_with_character_bound lb ub)
+let serialize_asn1_printable_string_TLV_with_character_bound lb ub
 = serialize_asn1_string_TLV_with_character_bound
     (PRINTABLE_STRING)
     (dfst)
