src/riot/asn1/ASN1.Spec.Value.SEQUENCE.fst
@@ -7,70 +7,14 @@ open ASN1.Spec.Tag
 open ASN1.Spec.Length
 open ASN1.Spec.Value.Envelop
 
-unfold
-let inbound_sequence_value_of
-  (#k: parser_kind)
-  (#t: Type0)
-  (#p: parser k t)
-  (s: serializer p)
-= inbound_envelop_tag_with_value_of SEQUENCE s
-
-let parse_asn1_sequence_TLV
-  (#k: parser_kind)
-  (#t: Type0)
-  (#p: parser k t)
-  (s: serializer p)
-: parser (parse_asn1_envelop_tag_with_TLV_kind SEQUENCE) (inbound_sequence_value_of s)
+let parse_asn1_sequence_TLV #k #t #p s
 = parse_asn1_envelop_tag_with_TLV SEQUENCE s
 
-let serialize_asn1_sequence_TLV
-  (#k: parser_kind)
-  (#t: Type0)
-  (#p: parser k t)
-  (s: serializer p)
-: serializer (parse_asn1_sequence_TLV s)
+let serialize_asn1_sequence_TLV #k #t #p s
 = serialize_asn1_envelop_tag_with_TLV SEQUENCE s
 
-unfold
-let predicate_serialize_asn1_sequence_TLV_unfold
-  (#k: parser_kind)
-  (#t: Type0)
-  (#p: parser k t)
-  (s: serializer p)
-= predicate_serialize_asn1_envelop_tag_with_TLV_unfold SEQUENCE s
-
-unfold
-let lemma_serialize_asn1_sequence_TLV_unfold
-  (#k: parser_kind)
-  (#t: Type0)
-  (#p: parser k t)
-  (s: serializer p)
-  (x: inbound_sequence_value_of s)
-: Lemma ( predicate_serialize_asn1_sequence_TLV_unfold s x )
+let lemma_serialize_asn1_sequence_TLV_unfold #k #t #p s x
 = lemma_serialize_asn1_envelop_tag_with_TLV_unfold SEQUENCE s x
 
-unfold
-let predicate_serialize_asn1_sequence_TLV_size
-  (#k: parser_kind)
-  (#t: Type0)
-  (#p: parser k t)
-  (s: serializer p)
-= predicate_serialize_asn1_envelop_tag_with_TLV_size SEQUENCE s
-
-unfold
-let lemma_serialize_asn1_sequence_TLV_size
-  (#k: parser_kind)
-  (#t: Type0)
-  (#p: parser k t)
-  (s: serializer p)
-  (x: inbound_sequence_value_of s)
-: Lemma ( predicate_serialize_asn1_sequence_TLV_size s x )
+let lemma_serialize_asn1_sequence_TLV_size #k #t #p s x
 = lemma_serialize_asn1_envelop_tag_with_TLV_size SEQUENCE s x
-
-unfold noextract
-let length_of_asn1_sequence_TLV
-  (#k: parser_kind)
-  (#t: Type0)
-  (#p: parser k t)
-  (s: serializer p)
-= length_of_asn1_envelop_tag_with_TLV SEQUENCE s
