src/riot/asn1/ASN1.Spec.Value.StringCombinator.fst
@@ -11,44 +11,14 @@ open FStar.Integers
 
 module B32 = FStar.Bytes
 
-noextract
-let parse_asn1_string
-  (t: asn1_type { t == IA5_STRING \/ t == PRINTABLE_STRING \/ t == OCTET_STRING })
-  (len_of_string: datatype_of_asn1_type t -> asn1_value_int32_of_type t)
-  (filter_string: (len: asn1_value_int32_of_type t)
-                  -> (s32: B32.lbytes32 len)
-                  -> GTot (bool))
-  (synth_string: (len: asn1_value_int32_of_type t)
-                 -> (s32: parse_filter_refine (filter_string len))
-                 -> GTot (x: datatype_of_asn1_type t
-                                  { len_of_string x== len }))
-  (prf: unit { forall len. synth_injective (synth_string len) })
-  (len: asn1_value_int32_of_type t)
-: parser _ (x: datatype_of_asn1_type t {len_of_string x == len})
+let parse_asn1_string t len_of_string filter_string synth_string prf len
 = parse_flbytes (v len)
   `parse_filter`
   filter_string len
   `parse_synth`
   synth_string len
 
-noextract
-let serialize_asn1_string
-  (t: asn1_type { t == IA5_STRING \/ t == PRINTABLE_STRING \/ t == OCTET_STRING })
-  (len_of_string: datatype_of_asn1_type t -> asn1_value_int32_of_type t)
-  (filter_string: (len: asn1_value_int32_of_type t)
-                  -> (s32: B32.lbytes32 len)
-                  -> GTot (bool))
-  (synth_string: (len: asn1_value_int32_of_type t)
-                 -> (s32: parse_filter_refine (filter_string len))
-                 -> GTot (x: datatype_of_asn1_type t
-                            { len_of_string x== len }))
-  (synth_string_inverse: (len: asn1_value_int32_of_type t)
-                         -> (x: datatype_of_asn1_type t { len_of_string x== len })
-                         -> (s32: parse_filter_refine (filter_string len)
-                                 { x == synth_string len s32 }))
-  (prf: unit { forall len. synth_injective (synth_string len) })
-  (len: asn1_value_int32_of_type t)
-: serializer (parse_asn1_string t len_of_string filter_string synth_string prf len)
+let serialize_asn1_string t len_of_string filter_string synth_string synth_string_inverse prf len
 = serialize_synth
   (* p1 *) (parse_flbytes (v len)
             `parse_filter`
@@ -60,47 +30,8 @@ let serialize_asn1_string
   (* g1 *) (synth_string_inverse len)
   (* Prf*) (prf)
 
-let predicate_serialize_asn1_string_unfold
-  (t: asn1_type { t == IA5_STRING \/ t == PRINTABLE_STRING \/ t == OCTET_STRING })
-  (len_of_string: datatype_of_asn1_type t -> asn1_value_int32_of_type t)
-  (filter_string: (len: asn1_value_int32_of_type t)
-                  -> (s32: B32.lbytes32 len)
-                  -> GTot (bool))
-  (synth_string: (len: asn1_value_int32_of_type t)
-                 -> (s32: parse_filter_refine (filter_string len))
-                 -> GTot (x: datatype_of_asn1_type t
-                            { len_of_string x== len }))
-  (synth_string_inverse: (len: asn1_value_int32_of_type t)
-                         -> (x: datatype_of_asn1_type t { len_of_string x== len })
-                         -> (s32: parse_filter_refine (filter_string len)
-                                 { x == synth_string len s32 }))
-  (prf: unit { forall len. synth_injective (synth_string len) })
-  (len: asn1_value_int32_of_type t)
-  (x: datatype_of_asn1_type t { len_of_string x== len })
-: Type0
-= serialize (serialize_asn1_string t len_of_string filter_string synth_string synth_string_inverse prf len) x
-  == serialize (serialize_flbytes (v len)) (synth_string_inverse len x)
 
-let lemma_serialize_asn1_string_unfold
-  (t: asn1_type { t == IA5_STRING \/ t == PRINTABLE_STRING \/ t == OCTET_STRING })
-  (len_of_string: datatype_of_asn1_type t -> asn1_value_int32_of_type t)
-  (filter_string: (len: asn1_value_int32_of_type t)
-                  -> (s32: B32.lbytes32 len)
-                  -> GTot (bool))
-  (synth_string: (len: asn1_value_int32_of_type t)
-                 -> (s32: parse_filter_refine (filter_string len))
-                 -> GTot (x: datatype_of_asn1_type t
-                            { len_of_string x== len }))
-  (synth_string_inverse: (len: asn1_value_int32_of_type t)
-                         -> (x: datatype_of_asn1_type t { len_of_string x== len })
-                         -> (s32: parse_filter_refine (filter_string len)
-                                 { x == synth_string len s32 }))
-  (prf: unit { forall len. synth_injective (synth_string len) })
-  (len: asn1_value_int32_of_type t)
-  (x: datatype_of_asn1_type t { len_of_string x== len })
-: Lemma (
-  predicate_serialize_asn1_string_unfold t len_of_string filter_string synth_string synth_string_inverse prf len x
-)
+let lemma_serialize_asn1_string_unfold t len_of_string filter_string synth_string synth_string_inverse prf len x
 = serialize_synth_eq
   (* p1 *) (parse_flbytes (v len)
             `parse_filter`
@@ -113,114 +44,27 @@ let lemma_serialize_asn1_string_unfold
   (* Prf*) (prf)
   (* in *) (x)
 
-let predicate_serialize_asn1_string_size
-  (t: asn1_type { t == IA5_STRING \/ t == PRINTABLE_STRING \/ t == OCTET_STRING })
-  (len_of_string: datatype_of_asn1_type t -> asn1_value_int32_of_type t)
-  (filter_string: (len: asn1_value_int32_of_type t)
-                  -> (s32: B32.lbytes32 len)
-                  -> GTot (bool))
-  (synth_string: (len: asn1_value_int32_of_type t)
-                 -> (s32: parse_filter_refine (filter_string len))
-                 -> GTot (x: datatype_of_asn1_type t
-                            { len_of_string x== len }))
-  (synth_string_inverse: (len: asn1_value_int32_of_type t)
-                         -> (x: datatype_of_asn1_type t { len_of_string x== len })
-                         -> (s32: parse_filter_refine (filter_string len)
-                                 { x == synth_string len s32 }))
-  (prf: unit { forall len. synth_injective (synth_string len) })
-  (len: asn1_value_int32_of_type t)
-  (x: datatype_of_asn1_type t { len_of_string x== len })
-: Type0
-= let length = length_of_opaque_serialization (serialize_asn1_string t len_of_string filter_string synth_string synth_string_inverse prf len) x in
-  length == v len /\
-  len == len_of_string x /\
-  asn1_value_length_inbound_of_type t length
-
-let lemma_serialize_asn1_string_size
-  (t: asn1_type { t == IA5_STRING \/ t == PRINTABLE_STRING \/ t == OCTET_STRING })
-  (len_of_string: datatype_of_asn1_type t -> asn1_value_int32_of_type t)
-  (filter_string: (len: asn1_value_int32_of_type t)
-                  -> (s32: B32.lbytes32 len)
-                  -> GTot (bool))
-  (synth_string: (len: asn1_value_int32_of_type t)
-                 -> (s32: parse_filter_refine (filter_string len))
-                 -> GTot (x: datatype_of_asn1_type t
-                            { len_of_string x== len }))
-  (synth_string_inverse: (len: asn1_value_int32_of_type t)
-                         -> (x: datatype_of_asn1_type t { len_of_string x== len })
-                         -> (s32: parse_filter_refine (filter_string len)
-                                 { x == synth_string len s32 }))
-  (prf: unit { forall len. synth_injective (synth_string len) })
-  (len: asn1_value_int32_of_type t)
-  (x: datatype_of_asn1_type t { len_of_string x== len })
-: Lemma (
-  predicate_serialize_asn1_string_size t len_of_string filter_string synth_string synth_string_inverse prf len x
-)
+let lemma_serialize_asn1_string_size t len_of_string filter_string synth_string synth_string_inverse prf len x
 = lemma_serialize_asn1_string_unfold t len_of_string filter_string synth_string synth_string_inverse prf len x
 
-noextract inline_for_extraction
-let parser_tag_of_asn1_string
-  (t: asn1_type { t == IA5_STRING \/ t == PRINTABLE_STRING \/ t == OCTET_STRING })
-  (len_of_string: datatype_of_asn1_type t -> asn1_value_int32_of_type t)
-  (x: datatype_of_asn1_type t)
-: Tot (the_asn1_tag t `tuple2` asn1_value_int32_of_type t)
+let parser_tag_of_asn1_string t len_of_string x
 = (t, len_of_string x)
 
-let synth_asn1_string_V
-  (t: asn1_type { t == IA5_STRING \/ t == PRINTABLE_STRING \/ t == OCTET_STRING })
-  (len_of_string: datatype_of_asn1_type t -> asn1_value_int32_of_type t)
-  (tag: the_asn1_tag t `tuple2` asn1_value_int32_of_type t)
-  (value: datatype_of_asn1_type t { v (len_of_string value) == v (snd tag) })
-: GTot (refine_with_tag (parser_tag_of_asn1_string t len_of_string) tag)
+let synth_asn1_string_V t len_of_string tag value
 = value
 
 noextract inline_for_extraction
-let synth_asn1_string_V_inverse
-  (t: asn1_type { t == IA5_STRING \/ t == PRINTABLE_STRING \/ t == OCTET_STRING })
-  (len_of_string: datatype_of_asn1_type t -> asn1_value_int32_of_type t)
-  (tag: the_asn1_tag t `tuple2` asn1_value_int32_of_type t)
-  (value': refine_with_tag (parser_tag_of_asn1_string t len_of_string) tag)
-: Tot (value: datatype_of_asn1_type t
-               { v (len_of_string value) == v (snd tag) /\
-                 value' == synth_asn1_string_V t len_of_string tag value })
+let synth_asn1_string_V_inverse t len_of_string tag value'
 = value'
 
-let parse_asn1_string_V
-  (t: asn1_type { t == IA5_STRING \/ t == PRINTABLE_STRING \/ t == OCTET_STRING })
-  (len_of_string: datatype_of_asn1_type t -> asn1_value_int32_of_type t)
-  (filter_string: (len: asn1_value_int32_of_type t)
-                  -> (s32: B32.lbytes32 len)
-                  -> GTot (bool))
-  (synth_string: (len: asn1_value_int32_of_type t)
-                       -> (s32: parse_filter_refine (filter_string len))
-                       -> GTot (x: datatype_of_asn1_type t
-                                  { len_of_string x== len }))
-  (prf: unit { forall len. synth_injective (synth_string len) })
-  (tag: the_asn1_tag t `tuple2` asn1_value_int32_of_type t)
-: parser (weak_kind_of_type t) (refine_with_tag (parser_tag_of_asn1_string t len_of_string) tag)
+let parse_asn1_string_V t len_of_string filter_string synth_string prf tag
 = weak_kind_of_type t
   `weaken`
   parse_asn1_string t len_of_string filter_string synth_string prf (snd tag)
   `parse_synth`
   synth_asn1_string_V t len_of_string tag
 
-let serialize_asn1_string_V
-  (t: asn1_type { t == IA5_STRING \/ t == PRINTABLE_STRING \/ t == OCTET_STRING })
-  (len_of_string: datatype_of_asn1_type t -> asn1_value_int32_of_type t)
-  (filter_string: (len: asn1_value_int32_of_type t)
-                  -> (s32: B32.lbytes32 len)
-                  -> GTot (bool))
-  (synth_string: (len: asn1_value_int32_of_type t)
-                 -> (s32: parse_filter_refine (filter_string len))
-                 -> GTot (x: datatype_of_asn1_type t
-                            { len_of_string x== len }))
-  (synth_string_inverse: (len: asn1_value_int32_of_type t)
-                         -> (x: datatype_of_asn1_type t { len_of_string x== len })
-                         -> (s32: parse_filter_refine (filter_string len)
-                                 { x == synth_string len s32 }))
-  (prf: unit { forall len. synth_injective (synth_string len) })
-  (tag: the_asn1_tag t `tuple2` asn1_value_int32_of_type t)
-: serializer (parse_asn1_string_V t len_of_string filter_string synth_string prf tag)
+let serialize_asn1_string_V t len_of_string filter_string synth_string synth_string_inverse prf tag
 = serialize_synth
   (* p1 *) (weak_kind_of_type t
             `weaken`
@@ -265,27 +109,7 @@ let lemma_serialize_asn1_string_V_unfold
   (* prf*) (prf)
   (* in *) (x)
 
-let parse_asn1_string_TLV_kind
-  (t: asn1_type { t == IA5_STRING \/ t == PRINTABLE_STRING \/ t == OCTET_STRING })
-: parser_kind
-= parse_asn1_tag_kind
-  `and_then_kind`
-  parse_asn1_length_kind_of_type t
-  `and_then_kind`
-  weak_kind_of_type t
-
-let parse_asn1_string_TLV
-  (t: asn1_type { t == IA5_STRING \/ t == PRINTABLE_STRING \/ t == OCTET_STRING })
-  (len_of_string: datatype_of_asn1_type t -> asn1_value_int32_of_type t)
-  (filter_string: (len: asn1_value_int32_of_type t)
-                  -> (s32: B32.lbytes32 len)
-                  -> GTot (bool))
-  (synth_string: (len: asn1_value_int32_of_type t)
-                       -> (s32: parse_filter_refine (filter_string len))
-                       -> GTot (x: datatype_of_asn1_type t
-                                  { len_of_string x== len }))
-  (prf: unit { forall len. synth_injective (synth_string len) })
-: parser (parse_asn1_string_TLV_kind t) (datatype_of_asn1_type t)
+let parse_asn1_string_TLV t len_of_string filter_string synth_string prf
 = parse_tagged_union
   (* pt *) (parse_asn1_tag_of_type t
             `nondep_then`
@@ -293,22 +117,7 @@ let parse_asn1_string_TLV
   (* tg *) (parser_tag_of_asn1_string t len_of_string)
   (* p  *) (parse_asn1_string_V t len_of_string filter_string synth_string prf)
 
-let serialize_asn1_string_TLV
-  (t: asn1_type { t == IA5_STRING \/ t == PRINTABLE_STRING \/ t == OCTET_STRING })
-  (len_of_string: datatype_of_asn1_type t -> asn1_value_int32_of_type t)
-  (filter_string: (len: asn1_value_int32_of_type t)
-                  -> (s32: B32.lbytes32 len)
-                  -> GTot (bool))
-  (synth_string: (len: asn1_value_int32_of_type t)
-                       -> (s32: parse_filter_refine (filter_string len))
-                       -> GTot (x: datatype_of_asn1_type t
-                                  { len_of_string x== len }))
-  (synth_string_inverse: (len: asn1_value_int32_of_type t)
-                         -> (x: datatype_of_asn1_type t { len_of_string x== len })
-                         -> (s32: parse_filter_refine (filter_string len)
-                                 { x == synth_string len s32 }))
-  (prf: unit { forall len. synth_injective (synth_string len) })
-: serializer (parse_asn1_string_TLV t len_of_string filter_string synth_string prf)
+let serialize_asn1_string_TLV t len_of_string filter_string synth_string synth_string_inverse prf
 = serialize_tagged_union
   (* st *) (serialize_asn1_tag_of_type t
             `serialize_nondep_then`
@@ -317,49 +126,7 @@ let serialize_asn1_string_TLV
   (* s  *) (serialize_asn1_string_V t len_of_string filter_string synth_string synth_string_inverse prf)
 
 #push-options "--z3rlimit 32"
-let predicate_serialize_asn1_string_TLV_unfold
-  (t: asn1_type { t == IA5_STRING \/ t == PRINTABLE_STRING \/ t == OCTET_STRING })
-  (len_of_string: datatype_of_asn1_type t -> asn1_value_int32_of_type t)
-  (filter_string: (len: asn1_value_int32_of_type t)
-                  -> (s32: B32.lbytes32 len)
-                  -> GTot (bool))
-  (synth_string: (len: asn1_value_int32_of_type t)
-                       -> (s32: parse_filter_refine (filter_string len))
-                       -> GTot (x: datatype_of_asn1_type t
-                                  { len_of_string x== len }))
-  (synth_string_inverse: (len: asn1_value_int32_of_type t)
-                         -> (x: datatype_of_asn1_type t { len_of_string x== len })
-                         -> (s32: parse_filter_refine (filter_string len)
-                                 { x == synth_string len s32 }))
-  (prf: unit { forall len. synth_injective (synth_string len) })
-  (x: datatype_of_asn1_type t)
-: Type0
-= serialize (serialize_asn1_string_TLV t len_of_string filter_string synth_string synth_string_inverse prf) x ==
-  serialize (serialize_asn1_tag_of_type t) t
-  `Seq.append`
-  serialize (serialize_asn1_length_of_type t) (len_of_string x)
-  `Seq.append`
-  serialize (serialize_asn1_string t len_of_string filter_string synth_string synth_string_inverse prf (len_of_string x)) x
-
-let lemma_serialize_asn1_string_TLV_unfold
-  (t: asn1_type { t == IA5_STRING \/ t == PRINTABLE_STRING \/ t == OCTET_STRING })
-  (len_of_string: datatype_of_asn1_type t -> asn1_value_int32_of_type t)
-  (filter_string: (len: asn1_value_int32_of_type t)
-                  -> (s32: B32.lbytes32 len)
-                  -> GTot (bool))
-  (synth_string: (len: asn1_value_int32_of_type t)
-                       -> (s32: parse_filter_refine (filter_string len))
-                       -> GTot (x: datatype_of_asn1_type t
-                                  { len_of_string x== len }))
-  (synth_string_inverse: (len: asn1_value_int32_of_type t)
-                         -> (x: datatype_of_asn1_type t { len_of_string x== len })
-                         -> (s32: parse_filter_refine (filter_string len)
-                                 { x == synth_string len s32 }))
-  (prf: unit { forall len. synth_injective (synth_string len) })
-  (x: datatype_of_asn1_type t)
-: Lemma (
-  predicate_serialize_asn1_string_TLV_unfold t len_of_string filter_string synth_string synth_string_inverse prf x
-)
+let lemma_serialize_asn1_string_TLV_unfold t len_of_string filter_string synth_string synth_string_inverse prf x
 = serialize_nondep_then_eq
   (* s1 *) (serialize_asn1_tag_of_type t)
   (* s2 *) (serialize_asn1_length_of_type t)
@@ -373,46 +140,8 @@ let lemma_serialize_asn1_string_TLV_unfold
   (* s  *) (serialize_asn1_string_V t len_of_string filter_string synth_string synth_string_inverse prf)
   (* in *) (x)
 
-let predicate_serialize_asn1_string_TLV_size
-  (t: asn1_type { t == IA5_STRING \/ t == PRINTABLE_STRING \/ t == OCTET_STRING })
-  (len_of_string: datatype_of_asn1_type t -> asn1_value_int32_of_type t)
-  (filter_string: (len: asn1_value_int32_of_type t)
-                  -> (s32: B32.lbytes32 len)
-                  -> GTot (bool))
-  (synth_string: (len: asn1_value_int32_of_type t)
-                       -> (s32: parse_filter_refine (filter_string len))
-                       -> GTot (x: datatype_of_asn1_type t
-                                  { len_of_string x== len }))
-  (synth_string_inverse: (len: asn1_value_int32_of_type t)
-                         -> (x: datatype_of_asn1_type t { len_of_string x== len })
-                         -> (s32: parse_filter_refine (filter_string len)
-                                 { x == synth_string len s32 }))
-  (prf: unit { forall len. synth_injective (synth_string len) })
-  (x: datatype_of_asn1_type t)
-: Type0
-= let length: nat = length_of_opaque_serialization (serialize_asn1_string_TLV t len_of_string filter_string synth_string synth_string_inverse prf) x in
-  length == 1 + length_of_asn1_length (len_of_string x) + v (len_of_string x) /\
-  asn1_TLV_length_inbound_of_type t length
 
-let lemma_serialize_asn1_string_TLV_size
-  (t: asn1_type { t == IA5_STRING \/ t == PRINTABLE_STRING \/ t == OCTET_STRING })
-  (len_of_string: datatype_of_asn1_type t -> asn1_value_int32_of_type t)
-  (filter_string: (len: asn1_value_int32_of_type t)
-                  -> (s32: B32.lbytes32 len)
-                  -> GTot (bool))
-  (synth_string: (len: asn1_value_int32_of_type t)
-                       -> (s32: parse_filter_refine (filter_string len))
-                       -> GTot (x: datatype_of_asn1_type t
-                                  { len_of_string x== len }))
-  (synth_string_inverse: (len: asn1_value_int32_of_type t)
-                         -> (x: datatype_of_asn1_type t { len_of_string x== len })
-                         -> (s32: parse_filter_refine (filter_string len)
-                                 { x == synth_string len s32 }))
-  (prf: unit { forall len. synth_injective (synth_string len) })
-  (x: datatype_of_asn1_type t)
-: Lemma (
-  predicate_serialize_asn1_string_TLV_size t len_of_string filter_string synth_string synth_string_inverse prf x
-)
+let lemma_serialize_asn1_string_TLV_size t len_of_string filter_string synth_string synth_string_inverse prf x
 = lemma_serialize_asn1_string_TLV_unfold t len_of_string filter_string synth_string synth_string_inverse prf x;
   lemma_serialize_asn1_tag_of_type_size t t;
   lemma_serialize_asn1_length_size (len_of_string x);
@@ -420,61 +149,15 @@ let lemma_serialize_asn1_string_TLV_size
   lemma_serialize_asn1_string_size t len_of_string filter_string synth_string synth_string_inverse prf (len_of_string x) x
 #pop-options
 
-let filter_asn1_string_with_character_bound
-  (t: asn1_type { t == IA5_STRING \/ t == PRINTABLE_STRING \/ t == OCTET_STRING })
-  (count_character: (x: datatype_of_asn1_type t) -> Tot (asn1_int32))
-  (lb: asn1_value_int32_of_type t)
-  (ub: asn1_value_int32_of_type t { lb <= ub })
-  (x: datatype_of_asn1_type t)
-: Tot (bool)
+let filter_asn1_string_with_character_bound t count_character lb ub x
 = lb <= count_character x && count_character x <= ub
 
-noextract inline_for_extraction
-let asn1_string_with_character_bound_t
-  (t: asn1_type { t == IA5_STRING \/ t == PRINTABLE_STRING \/ t == OCTET_STRING })
-  (count_character: (x: datatype_of_asn1_type t) -> Tot (asn1_int32))
-  (lb: asn1_value_int32_of_type t)
-  (ub: asn1_value_int32_of_type t { lb <= ub })
-= parse_filter_refine (filter_asn1_string_with_character_bound t count_character lb ub)
-
-let parse_asn1_string_TLV_with_character_bound
-  (t: asn1_type { t == IA5_STRING \/ t == PRINTABLE_STRING \/ t == OCTET_STRING })
-  (len_of_string: datatype_of_asn1_type t -> asn1_value_int32_of_type t)
-  (filter_string: (len: asn1_value_int32_of_type t)
-                  -> (s32: B32.lbytes32 len)
-                  -> GTot (bool))
-  (synth_string: (len: asn1_value_int32_of_type t)
-                       -> (s32: parse_filter_refine (filter_string len))
-                       -> GTot (x: datatype_of_asn1_type t
-                                  { len_of_string x== len }))
-  (prf: unit { forall len. synth_injective (synth_string len) })
-  (count_character: (x: datatype_of_asn1_type t) -> Tot (asn1_int32))
-  (lb: asn1_value_int32_of_type t)
-  (ub: asn1_value_int32_of_type t { lb <= ub })
-: parser (parse_asn1_string_TLV_kind t) (asn1_string_with_character_bound_t t count_character lb ub)
+let parse_asn1_string_TLV_with_character_bound t len_of_string filter_string synth_string prf count_character lb ub
 = parse_asn1_string_TLV t len_of_string filter_string synth_string prf
   `parse_filter`
   filter_asn1_string_with_character_bound t count_character lb ub
 
-let serialize_asn1_string_TLV_with_character_bound
-  (t: asn1_type { t == IA5_STRING \/ t == PRINTABLE_STRING \/ t == OCTET_STRING })
-  (len_of_string: datatype_of_asn1_type t -> asn1_value_int32_of_type t)
-  (filter_string: (len: asn1_value_int32_of_type t)
-                  -> (s32: B32.lbytes32 len)
-                  -> GTot (bool))
-  (synth_string: (len: asn1_value_int32_of_type t)
-                       -> (s32: parse_filter_refine (filter_string len))
-                       -> GTot (x: datatype_of_asn1_type t
-                                  { len_of_string x== len }))
-  (synth_string_inverse: (len: asn1_value_int32_of_type t)
-                         -> (x: datatype_of_asn1_type t { len_of_string x== len })
-                         -> (s32: parse_filter_refine (filter_string len)
-                                 { x == synth_string len s32 }))
-  (prf: unit { forall len. synth_injective (synth_string len) })
-  (count_character: (x: datatype_of_asn1_type t) -> Tot (asn1_int32))
-  (lb: asn1_value_int32_of_type t)
-  (ub: asn1_value_int32_of_type t { lb <= ub })
-: serializer (parse_asn1_string_TLV_with_character_bound t len_of_string filter_string synth_string prf count_character lb ub)
+let serialize_asn1_string_TLV_with_character_bound t len_of_string filter_string synth_string synth_string_inverse prf count_character lb ub
 = serialize_asn1_string_TLV t len_of_string filter_string synth_string synth_string_inverse prf
   `serialize_filter`
   filter_asn1_string_with_character_bound t count_character lb ub
