src/riot/asn1/ASN1.Low.Value.PRINTABLE_STRING.fsti
@@ -1,0 +1,17 @@
+module ASN1.Low.Value.PRINTABLE_STRING
+
+open ASN1.Base
+open ASN1.Spec.Value.PRINTABLE_STRING
+open ASN1.Low.Base
+
+open FStar.Integers
+
+inline_for_extraction noextract
+val serialize32_asn1_printable_string_TLV_backwards
+: serializer32_backwards (serialize_asn1_printable_string_TLV)
+
+inline_for_extraction noextract
+val serialize32_asn1_printable_string_TLV_with_character_bound_backwards
+  (lb: asn1_value_int32_of_type PRINTABLE_STRING)
+  (ub: asn1_value_int32_of_type PRINTABLE_STRING { lb <= ub })
+: serializer32_backwards (serialize_asn1_printable_string_TLV_with_character_bound lb ub)
