src/riot/asn1/ASN1.Low.Value.SEQUENCE.fsti
@@ -1,0 +1,16 @@
+module ASN1.Low.Value.SEQUENCE
+///
+/// ASN.1 Low
+open LowParse.Low.Base
+
+open ASN1.Base
+open ASN1.Spec.Value.SEQUENCE
+open ASN1.Low.Base
+
+val serialize32_asn1_sequence_TLV_backwards
+  (#k: parser_kind)
+  (#t: Type0)
+  (#p: parser k t)
+  (#s: serializer p)
+  (s32: serializer32_backwards s)
+: (serializer32_backwards (serialize_asn1_sequence_TLV s))
