src/riot/asn1/ASN1.Low.Value.StringCombinator.fsti
@@ -1,0 +1,68 @@
+module ASN1.Low.Value.StringCombinator
+
+open ASN1.Base
+open ASN1.Spec.Value.StringCombinator
+open ASN1.Low.Base
+
+open FStar.Integers
+
+module B32 = FStar.Bytes
+
+noextract inline_for_extraction
+val serialize32_asn1_string_backwards
+  (t: asn1_type { t == IA5_STRING \/ t == PRINTABLE_STRING \/ t == OCTET_STRING })
+  (len_of_string: datatype_of_asn1_type t -> asn1_value_int32_of_type t)
+  (filter_string: (len: asn1_value_int32_of_type t)
+                  -> (s32: B32.lbytes32 len)
+                  -> GTot (bool))
+  (synth_string: (len: asn1_value_int32_of_type t)
+                 -> (s32: parse_filter_refine (filter_string len))
+                 -> GTot (x: datatype_of_asn1_type t
+                            { len_of_string x== len }))
+  (synth_string_inverse: (len: asn1_value_int32_of_type t)
+                         -> (x: datatype_of_asn1_type t { len_of_string x== len })
+                         -> (s32: parse_filter_refine (filter_string len)
+                                 { x == synth_string len s32 }))
+  (prf: unit { forall len. synth_injective (synth_string len) })
+  (len: asn1_value_int32_of_type t)
+: (serializer32_backwards (serialize_asn1_string t len_of_string filter_string synth_string synth_string_inverse prf len))
+
+#push-options "--z3rlimit 32 --fuel 2 --ifuel 2"
+noextract inline_for_extraction
+val serialize32_asn1_string_TLV_backwards
+  (t: asn1_type { t == IA5_STRING \/ t == PRINTABLE_STRING \/ t == OCTET_STRING })
+  (len_of_string: datatype_of_asn1_type t -> asn1_value_int32_of_type t)
+  (filter_string: (len: asn1_value_int32_of_type t)
+                  -> (s32: B32.lbytes32 len)
+                  -> GTot (bool))
+  (synth_string: (len: asn1_value_int32_of_type t)
+                       -> (s32: parse_filter_refine (filter_string len))
+                       -> GTot (x: datatype_of_asn1_type t
+                                  { len_of_string x== len }))
+  (synth_string_inverse: (len: asn1_value_int32_of_type t)
+                         -> (x: datatype_of_asn1_type t { len_of_string x== len })
+                         -> (s32: parse_filter_refine (filter_string len)
+                                 { x == synth_string len s32 }))
+  (prf: unit { forall len. synth_injective (synth_string len) })
+: serializer32_backwards (serialize_asn1_string_TLV t len_of_string filter_string synth_string synth_string_inverse prf)
+
+noextract inline_for_extraction
+val serialize32_asn1_string_TLV_with_character_bound_backwards
+  (t: asn1_type { t == IA5_STRING \/ t == PRINTABLE_STRING \/ t == OCTET_STRING })
+  (len_of_string: datatype_of_asn1_type t -> asn1_value_int32_of_type t)
+  (filter_string: (len: asn1_value_int32_of_type t)
+                  -> (s32: B32.lbytes32 len)
+                  -> GTot (bool))
+  (synth_string: (len: asn1_value_int32_of_type t)
+                       -> (s32: parse_filter_refine (filter_string len))
+                       -> GTot (x: datatype_of_asn1_type t
+                                  { len_of_string x== len }))
+  (synth_string_inverse: (len: asn1_value_int32_of_type t)
+                         -> (x: datatype_of_asn1_type t { len_of_string x== len })
+                         -> (s32: parse_filter_refine (filter_string len)
+                                 { x == synth_string len s32 }))
+  (prf: unit { forall len. synth_injective (synth_string len) })
+  (count_character: (x: datatype_of_asn1_type t) -> Tot (asn1_int32))
+  (lb: asn1_value_int32_of_type t)
+  (ub: asn1_value_int32_of_type t { lb <= ub })
+: serializer32_backwards (serialize_asn1_string_TLV_with_character_bound t len_of_string filter_string synth_string synth_string_inverse prf count_character lb ub)
