src/riot/asn1/ASN1.Spec.Value.SEQUENCE.fsti
@@ -1,0 +1,68 @@
+module ASN1.Spec.Value.SEQUENCE
+
+open ASN1.Spec.Base
+
+open ASN1.Base
+open ASN1.Spec.Value.Envelop
+
+unfold
+let inbound_sequence_value_of
+  (#k: parser_kind)
+  (#t: Type0)
+  (#p: parser k t)
+  (s: serializer p)
+= inbound_envelop_tag_with_value_of SEQUENCE s
+
+val parse_asn1_sequence_TLV
+  (#k: parser_kind)
+  (#t: Type0)
+  (#p: parser k t)
+  (s: serializer p)
+: parser (parse_asn1_envelop_tag_with_TLV_kind SEQUENCE) (inbound_sequence_value_of s)
+
+val serialize_asn1_sequence_TLV
+  (#k: parser_kind)
+  (#t: Type0)
+  (#p: parser k t)
+  (s: serializer p)
+: serializer (parse_asn1_sequence_TLV s)
+
+unfold
+let predicate_serialize_asn1_sequence_TLV_unfold
+  (#k: parser_kind)
+  (#t: Type0)
+  (#p: parser k t)
+  (s: serializer p)
+= predicate_serialize_asn1_envelop_tag_with_TLV_unfold SEQUENCE s
+
+val lemma_serialize_asn1_sequence_TLV_unfold
+  (#k: parser_kind)
+  (#t: Type0)
+  (#p: parser k t)
+  (s: serializer p)
+  (x: inbound_sequence_value_of s)
+: Lemma ( predicate_serialize_asn1_sequence_TLV_unfold s x )
+
+unfold
+let predicate_serialize_asn1_sequence_TLV_size
+  (#k: parser_kind)
+  (#t: Type0)
+  (#p: parser k t)
+  (s: serializer p)
+= predicate_serialize_asn1_envelop_tag_with_TLV_size SEQUENCE s
+
+val lemma_serialize_asn1_sequence_TLV_size
+  (#k: parser_kind)
+  (#t: Type0)
+  (#p: parser k t)
+  (s: serializer p)
+  (x: inbound_sequence_value_of s)
+: Lemma ( predicate_serialize_asn1_sequence_TLV_size s x )
+
+unfold noextract
+let length_of_asn1_sequence_TLV
+  (#k: parser_kind)
+  (#t: Type0)
+  (#p: parser k t)
+  (s: serializer p)
+= length_of_asn1_envelop_tag_with_TLV SEQUENCE s
