src/riot/asn1/ASN1.Spec.Value.StringCombinator.fsti
@@ -1,0 +1,371 @@
+module ASN1.Spec.Value.StringCombinator
+
+open ASN1.Spec.Base
+open LowParse.Spec.Bytes
+
+open ASN1.Base
+open ASN1.Spec.Tag
+open ASN1.Spec.Length
+
+open FStar.Integers
+
+module B32 = FStar.Bytes
+
+noextract
+val parse_asn1_string
+  (t: asn1_type { t == IA5_STRING \/ t == PRINTABLE_STRING \/ t == OCTET_STRING })
+  (len_of_string: datatype_of_asn1_type t -> asn1_value_int32_of_type t)
+  (filter_string: (len: asn1_value_int32_of_type t)
+                  -> (s32: B32.lbytes32 len)
+                  -> GTot (bool))
+  (synth_string: (len: asn1_value_int32_of_type t)
+                 -> (s32: parse_filter_refine (filter_string len))
+                 -> GTot (x: datatype_of_asn1_type t
+                                  { len_of_string x== len }))
+  (prf: unit { forall len. synth_injective (synth_string len) })
+  (len: asn1_value_int32_of_type t)
+: parser (parse_filter_kind (total_constant_size_parser_kind (v len)))
+    (x: datatype_of_asn1_type t {len_of_string x == len})
+
+noextract
+val serialize_asn1_string
+  (t: asn1_type { t == IA5_STRING \/ t == PRINTABLE_STRING \/ t == OCTET_STRING })
+  (len_of_string: datatype_of_asn1_type t -> asn1_value_int32_of_type t)
+  (filter_string: (len: asn1_value_int32_of_type t)
+                  -> (s32: B32.lbytes32 len)
+                  -> GTot (bool))
+  (synth_string: (len: asn1_value_int32_of_type t)
+                 -> (s32: parse_filter_refine (filter_string len))
+                 -> GTot (x: datatype_of_asn1_type t
+                            { len_of_string x== len }))
+  (synth_string_inverse: (len: asn1_value_int32_of_type t)
+                         -> (x: datatype_of_asn1_type t { len_of_string x== len })
+                         -> (s32: parse_filter_refine (filter_string len)
+                                 { x == synth_string len s32 }))
+  (prf: unit { forall len. synth_injective (synth_string len) })
+  (len: asn1_value_int32_of_type t)
+: serializer (parse_asn1_string t len_of_string filter_string synth_string prf len)
+
+unfold
+let predicate_serialize_asn1_string_unfold
+  (t: asn1_type { t == IA5_STRING \/ t == PRINTABLE_STRING \/ t == OCTET_STRING })
+  (len_of_string: datatype_of_asn1_type t -> asn1_value_int32_of_type t)
+  (filter_string: (len: asn1_value_int32_of_type t)
+                  -> (s32: B32.lbytes32 len)
+                  -> GTot (bool))
+  (synth_string: (len: asn1_value_int32_of_type t)
+                 -> (s32: parse_filter_refine (filter_string len))
+                 -> GTot (x: datatype_of_asn1_type t
+                            { len_of_string x== len }))
+  (synth_string_inverse: (len: asn1_value_int32_of_type t)
+                         -> (x: datatype_of_asn1_type t { len_of_string x== len })
+                         -> (s32: parse_filter_refine (filter_string len)
+                                 { x == synth_string len s32 }))
+  (prf: unit { forall len. synth_injective (synth_string len) })
+  (len: asn1_value_int32_of_type t)
+  (x: datatype_of_asn1_type t { len_of_string x== len })
+: Type0
+= serialize (serialize_asn1_string t len_of_string filter_string synth_string synth_string_inverse prf len) x
+  == serialize (serialize_flbytes (v len)) (synth_string_inverse len x)
+
+val lemma_serialize_asn1_string_unfold
+  (t: asn1_type { t == IA5_STRING \/ t == PRINTABLE_STRING \/ t == OCTET_STRING })
+  (len_of_string: datatype_of_asn1_type t -> asn1_value_int32_of_type t)
+  (filter_string: (len: asn1_value_int32_of_type t)
+                  -> (s32: B32.lbytes32 len)
+                  -> GTot (bool))
+  (synth_string: (len: asn1_value_int32_of_type t)
+                 -> (s32: parse_filter_refine (filter_string len))
+                 -> GTot (x: datatype_of_asn1_type t
+                            { len_of_string x== len }))
+  (synth_string_inverse: (len: asn1_value_int32_of_type t)
+                         -> (x: datatype_of_asn1_type t { len_of_string x== len })
+                         -> (s32: parse_filter_refine (filter_string len)
+                                 { x == synth_string len s32 }))
+  (prf: unit { forall len. synth_injective (synth_string len) })
+  (len: asn1_value_int32_of_type t)
+  (x: datatype_of_asn1_type t { len_of_string x== len })
+: Lemma (
+  predicate_serialize_asn1_string_unfold t len_of_string filter_string synth_string synth_string_inverse prf len x
+)
+
+unfold
+let predicate_serialize_asn1_string_size
+  (t: asn1_type { t == IA5_STRING \/ t == PRINTABLE_STRING \/ t == OCTET_STRING })
+  (len_of_string: datatype_of_asn1_type t -> asn1_value_int32_of_type t)
+  (filter_string: (len: asn1_value_int32_of_type t)
+                  -> (s32: B32.lbytes32 len)
+                  -> GTot (bool))
+  (synth_string: (len: asn1_value_int32_of_type t)
+                 -> (s32: parse_filter_refine (filter_string len))
+                 -> GTot (x: datatype_of_asn1_type t
+                            { len_of_string x== len }))
+  (synth_string_inverse: (len: asn1_value_int32_of_type t)
+                         -> (x: datatype_of_asn1_type t { len_of_string x== len })
+                         -> (s32: parse_filter_refine (filter_string len)
+                                 { x == synth_string len s32 }))
+  (prf: unit { forall len. synth_injective (synth_string len) })
+  (len: asn1_value_int32_of_type t)
+  (x: datatype_of_asn1_type t { len_of_string x== len })
+: Type0
+= let length = length_of_opaque_serialization (serialize_asn1_string t len_of_string filter_string synth_string synth_string_inverse prf len) x in
+  length == v len /\
+  len == len_of_string x /\
+  asn1_value_length_inbound_of_type t length
+
+val lemma_serialize_asn1_string_size
+  (t: asn1_type { t == IA5_STRING \/ t == PRINTABLE_STRING \/ t == OCTET_STRING })
+  (len_of_string: datatype_of_asn1_type t -> asn1_value_int32_of_type t)
+  (filter_string: (len: asn1_value_int32_of_type t)
+                  -> (s32: B32.lbytes32 len)
+                  -> GTot (bool))
+  (synth_string: (len: asn1_value_int32_of_type t)
+                 -> (s32: parse_filter_refine (filter_string len))
+                 -> GTot (x: datatype_of_asn1_type t
+                            { len_of_string x== len }))
+  (synth_string_inverse: (len: asn1_value_int32_of_type t)
+                         -> (x: datatype_of_asn1_type t { len_of_string x== len })
+                         -> (s32: parse_filter_refine (filter_string len)
+                                 { x == synth_string len s32 }))
+  (prf: unit { forall len. synth_injective (synth_string len) })
+  (len: asn1_value_int32_of_type t)
+  (x: datatype_of_asn1_type t { len_of_string x== len })
+: Lemma (
+  predicate_serialize_asn1_string_size t len_of_string filter_string synth_string synth_string_inverse prf len x
+)
+
+noextract inline_for_extraction
+val parser_tag_of_asn1_string
+  (t: asn1_type { t == IA5_STRING \/ t == PRINTABLE_STRING \/ t == OCTET_STRING })
+  (len_of_string: datatype_of_asn1_type t -> asn1_value_int32_of_type t)
+  (x: datatype_of_asn1_type t)
+: Tot (the_asn1_tag t `tuple2` asn1_value_int32_of_type t)
+
+val synth_asn1_string_V
+  (t: asn1_type { t == IA5_STRING \/ t == PRINTABLE_STRING \/ t == OCTET_STRING })
+  (len_of_string: datatype_of_asn1_type t -> asn1_value_int32_of_type t)
+  (tag: the_asn1_tag t `tuple2` asn1_value_int32_of_type t)
+  (value: datatype_of_asn1_type t { v (len_of_string value) == v (snd tag) })
+: GTot (refine_with_tag (parser_tag_of_asn1_string t len_of_string) tag)
+
+noextract inline_for_extraction
+val synth_asn1_string_V_inverse
+  (t: asn1_type { t == IA5_STRING \/ t == PRINTABLE_STRING \/ t == OCTET_STRING })
+  (len_of_string: datatype_of_asn1_type t -> asn1_value_int32_of_type t)
+  (tag: the_asn1_tag t `tuple2` asn1_value_int32_of_type t)
+  (value': refine_with_tag (parser_tag_of_asn1_string t len_of_string) tag)
+: Tot (value: datatype_of_asn1_type t
+               { v (len_of_string value) == v (snd tag) /\
+                 value' == synth_asn1_string_V t len_of_string tag value })
+
+val parse_asn1_string_V
+  (t: asn1_type { t == IA5_STRING \/ t == PRINTABLE_STRING \/ t == OCTET_STRING })
+  (len_of_string: datatype_of_asn1_type t -> asn1_value_int32_of_type t)
+  (filter_string: (len: asn1_value_int32_of_type t)
+                  -> (s32: B32.lbytes32 len)
+                  -> GTot (bool))
+  (synth_string: (len: asn1_value_int32_of_type t)
+                       -> (s32: parse_filter_refine (filter_string len))
+                       -> GTot (x: datatype_of_asn1_type t
+                                  { len_of_string x== len }))
+  (prf: unit { forall len. synth_injective (synth_string len) })
+  (tag: the_asn1_tag t `tuple2` asn1_value_int32_of_type t)
+: parser (weak_kind_of_type t) (refine_with_tag (parser_tag_of_asn1_string t len_of_string) tag)
+
+val serialize_asn1_string_V
+  (t: asn1_type { t == IA5_STRING \/ t == PRINTABLE_STRING \/ t == OCTET_STRING })
+  (len_of_string: datatype_of_asn1_type t -> asn1_value_int32_of_type t)
+  (filter_string: (len: asn1_value_int32_of_type t)
+                  -> (s32: B32.lbytes32 len)
+                  -> GTot (bool))
+  (synth_string: (len: asn1_value_int32_of_type t)
+                 -> (s32: parse_filter_refine (filter_string len))
+                 -> GTot (x: datatype_of_asn1_type t
+                            { len_of_string x== len }))
+  (synth_string_inverse: (len: asn1_value_int32_of_type t)
+                         -> (x: datatype_of_asn1_type t { len_of_string x== len })
+                         -> (s32: parse_filter_refine (filter_string len)
+                                 { x == synth_string len s32 }))
+  (prf: unit { forall len. synth_injective (synth_string len) })
+  (tag: the_asn1_tag t `tuple2` asn1_value_int32_of_type t)
+: serializer (parse_asn1_string_V t len_of_string filter_string synth_string prf tag)
+
+let parse_asn1_string_TLV_kind
+  (t: asn1_type { t == IA5_STRING \/ t == PRINTABLE_STRING \/ t == OCTET_STRING })
+: parser_kind
+= parse_asn1_tag_kind
+  `and_then_kind`
+  parse_asn1_length_kind_of_type t
+  `and_then_kind`
+  weak_kind_of_type t
+
+val parse_asn1_string_TLV
+  (t: asn1_type { t == IA5_STRING \/ t == PRINTABLE_STRING \/ t == OCTET_STRING })
+  (len_of_string: datatype_of_asn1_type t -> asn1_value_int32_of_type t)
+  (filter_string: (len: asn1_value_int32_of_type t)
+                  -> (s32: B32.lbytes32 len)
+                  -> GTot (bool))
+  (synth_string: (len: asn1_value_int32_of_type t)
+                       -> (s32: parse_filter_refine (filter_string len))
+                       -> GTot (x: datatype_of_asn1_type t
+                                  { len_of_string x== len }))
+  (prf: unit { forall len. synth_injective (synth_string len) })
+: parser (parse_asn1_string_TLV_kind t) (datatype_of_asn1_type t)
+
+val serialize_asn1_string_TLV
+  (t: asn1_type { t == IA5_STRING \/ t == PRINTABLE_STRING \/ t == OCTET_STRING })
+  (len_of_string: datatype_of_asn1_type t -> asn1_value_int32_of_type t)
+  (filter_string: (len: asn1_value_int32_of_type t)
+                  -> (s32: B32.lbytes32 len)
+                  -> GTot (bool))
+  (synth_string: (len: asn1_value_int32_of_type t)
+                       -> (s32: parse_filter_refine (filter_string len))
+                       -> GTot (x: datatype_of_asn1_type t
+                                  { len_of_string x== len }))
+  (synth_string_inverse: (len: asn1_value_int32_of_type t)
+                         -> (x: datatype_of_asn1_type t { len_of_string x== len })
+                         -> (s32: parse_filter_refine (filter_string len)
+                                 { x == synth_string len s32 }))
+  (prf: unit { forall len. synth_injective (synth_string len) })
+: serializer (parse_asn1_string_TLV t len_of_string filter_string synth_string prf)
+
+#push-options "--z3rlimit 32"
+unfold
+let predicate_serialize_asn1_string_TLV_unfold
+  (t: asn1_type { t == IA5_STRING \/ t == PRINTABLE_STRING \/ t == OCTET_STRING })
+  (len_of_string: datatype_of_asn1_type t -> asn1_value_int32_of_type t)
+  (filter_string: (len: asn1_value_int32_of_type t)
+                  -> (s32: B32.lbytes32 len)
+                  -> GTot (bool))
+  (synth_string: (len: asn1_value_int32_of_type t)
+                       -> (s32: parse_filter_refine (filter_string len))
+                       -> GTot (x: datatype_of_asn1_type t
+                                  { len_of_string x== len }))
+  (synth_string_inverse: (len: asn1_value_int32_of_type t)
+                         -> (x: datatype_of_asn1_type t { len_of_string x== len })
+                         -> (s32: parse_filter_refine (filter_string len)
+                                 { x == synth_string len s32 }))
+  (prf: unit { forall len. synth_injective (synth_string len) })
+  (x: datatype_of_asn1_type t)
+: Type0
+= serialize (serialize_asn1_string_TLV t len_of_string filter_string synth_string synth_string_inverse prf) x ==
+  serialize (serialize_asn1_tag_of_type t) t
+  `Seq.append`
+  serialize (serialize_asn1_length_of_type t) (len_of_string x)
+  `Seq.append`
+  serialize (serialize_asn1_string t len_of_string filter_string synth_string synth_string_inverse prf (len_of_string x)) x
+
+val lemma_serialize_asn1_string_TLV_unfold
+  (t: asn1_type { t == IA5_STRING \/ t == PRINTABLE_STRING \/ t == OCTET_STRING })
+  (len_of_string: datatype_of_asn1_type t -> asn1_value_int32_of_type t)
+  (filter_string: (len: asn1_value_int32_of_type t)
+                  -> (s32: B32.lbytes32 len)
+                  -> GTot (bool))
+  (synth_string: (len: asn1_value_int32_of_type t)
+                       -> (s32: parse_filter_refine (filter_string len))
+                       -> GTot (x: datatype_of_asn1_type t
+                                  { len_of_string x== len }))
+  (synth_string_inverse: (len: asn1_value_int32_of_type t)
+                         -> (x: datatype_of_asn1_type t { len_of_string x== len })
+                         -> (s32: parse_filter_refine (filter_string len)
+                                 { x == synth_string len s32 }))
+  (prf: unit { forall len. synth_injective (synth_string len) })
+  (x: datatype_of_asn1_type t)
+: Lemma (
+  predicate_serialize_asn1_string_TLV_unfold t len_of_string filter_string synth_string synth_string_inverse prf x
+)
+
+unfold
+let predicate_serialize_asn1_string_TLV_size
+  (t: asn1_type { t == IA5_STRING \/ t == PRINTABLE_STRING \/ t == OCTET_STRING })
+  (len_of_string: datatype_of_asn1_type t -> asn1_value_int32_of_type t)
+  (filter_string: (len: asn1_value_int32_of_type t)
+                  -> (s32: B32.lbytes32 len)
+                  -> GTot (bool))
+  (synth_string: (len: asn1_value_int32_of_type t)
+                       -> (s32: parse_filter_refine (filter_string len))
+                       -> GTot (x: datatype_of_asn1_type t
+                                  { len_of_string x== len }))
+  (synth_string_inverse: (len: asn1_value_int32_of_type t)
+                         -> (x: datatype_of_asn1_type t { len_of_string x== len })
+                         -> (s32: parse_filter_refine (filter_string len)
+                                 { x == synth_string len s32 }))
+  (prf: unit { forall len. synth_injective (synth_string len) })
+  (x: datatype_of_asn1_type t)
+: Type0
+= let length: nat = length_of_opaque_serialization (serialize_asn1_string_TLV t len_of_string filter_string synth_string synth_string_inverse prf) x in
+  length == 1 + length_of_asn1_length (len_of_string x) + v (len_of_string x) /\
+  asn1_TLV_length_inbound_of_type t length
+
+val  lemma_serialize_asn1_string_TLV_size
+  (t: asn1_type { t == IA5_STRING \/ t == PRINTABLE_STRING \/ t == OCTET_STRING })
+  (len_of_string: datatype_of_asn1_type t -> asn1_value_int32_of_type t)
+  (filter_string: (len: asn1_value_int32_of_type t)
+                  -> (s32: B32.lbytes32 len)
+                  -> GTot (bool))
+  (synth_string: (len: asn1_value_int32_of_type t)
+                       -> (s32: parse_filter_refine (filter_string len))
+                       -> GTot (x: datatype_of_asn1_type t
+                                  { len_of_string x== len }))
+  (synth_string_inverse: (len: asn1_value_int32_of_type t)
+                         -> (x: datatype_of_asn1_type t { len_of_string x== len })
+                         -> (s32: parse_filter_refine (filter_string len)
+                                 { x == synth_string len s32 }))
+  (prf: unit { forall len. synth_injective (synth_string len) })
+  (x: datatype_of_asn1_type t)
+: Lemma (
+  predicate_serialize_asn1_string_TLV_size t len_of_string filter_string synth_string synth_string_inverse prf x
+)
+#pop-options
+
+val filter_asn1_string_with_character_bound
+  (t: asn1_type { t == IA5_STRING \/ t == PRINTABLE_STRING \/ t == OCTET_STRING })
+  (count_character: (x: datatype_of_asn1_type t) -> Tot (asn1_int32))
+  (lb: asn1_value_int32_of_type t)
+  (ub: asn1_value_int32_of_type t { lb <= ub })
+  (x: datatype_of_asn1_type t)
+: Tot (bool)
+
+noextract inline_for_extraction unfold
+let asn1_string_with_character_bound_t
+  (t: asn1_type { t == IA5_STRING \/ t == PRINTABLE_STRING \/ t == OCTET_STRING })
+  (count_character: (x: datatype_of_asn1_type t) -> Tot (asn1_int32))
+  (lb: asn1_value_int32_of_type t)
+  (ub: asn1_value_int32_of_type t { lb <= ub })
+= parse_filter_refine (filter_asn1_string_with_character_bound t count_character lb ub)
+
+val parse_asn1_string_TLV_with_character_bound
+  (t: asn1_type { t == IA5_STRING \/ t == PRINTABLE_STRING \/ t == OCTET_STRING })
+  (len_of_string: datatype_of_asn1_type t -> asn1_value_int32_of_type t)
+  (filter_string: (len: asn1_value_int32_of_type t)
+                  -> (s32: B32.lbytes32 len)
+                  -> GTot (bool))
+  (synth_string: (len: asn1_value_int32_of_type t)
+                       -> (s32: parse_filter_refine (filter_string len))
+                       -> GTot (x: datatype_of_asn1_type t
+                                  { len_of_string x== len }))
+  (prf: unit { forall len. synth_injective (synth_string len) })
+  (count_character: (x: datatype_of_asn1_type t) -> Tot (asn1_int32))
+  (lb: asn1_value_int32_of_type t)
+  (ub: asn1_value_int32_of_type t { lb <= ub })
+: parser (parse_asn1_string_TLV_kind t) (asn1_string_with_character_bound_t t count_character lb ub)
+
+val serialize_asn1_string_TLV_with_character_bound
+  (t: asn1_type { t == IA5_STRING \/ t == PRINTABLE_STRING \/ t == OCTET_STRING })
+  (len_of_string: datatype_of_asn1_type t -> asn1_value_int32_of_type t)
+  (filter_string: (len: asn1_value_int32_of_type t)
+                  -> (s32: B32.lbytes32 len)
+                  -> GTot (bool))
+  (synth_string: (len: asn1_value_int32_of_type t)
+                       -> (s32: parse_filter_refine (filter_string len))
+                       -> GTot (x: datatype_of_asn1_type t
+                                  { len_of_string x== len }))
+  (synth_string_inverse: (len: asn1_value_int32_of_type t)
+                         -> (x: datatype_of_asn1_type t { len_of_string x== len })
+                         -> (s32: parse_filter_refine (filter_string len)
+                                 { x == synth_string len s32 }))
+  (prf: unit { forall len. synth_injective (synth_string len) })
+  (count_character: (x: datatype_of_asn1_type t) -> Tot (asn1_int32))
+  (lb: asn1_value_int32_of_type t)
+  (ub: asn1_value_int32_of_type t { lb <= ub })
+: serializer (parse_asn1_string_TLV_with_character_bound t len_of_string filter_string synth_string prf count_character lb ub)
